theories/heap_lang/lib/barrier/barrier.v
@@ -3,4 +3,4 @@ From iris.heap_lang Require Export notation.
 Definition newbarrier : val := λ: <>, ref #false.
 Definition signal : val := λ: "x", "x" <- #true.
 Definition wait : val :=
-  rec: "wait" "x" := if: !"x" then #() else "wait" "x".
+  rec: "wait" "x" := if: !"x" then () else "wait" "x".
