theories/heap_lang/lib/spawn.v
@@ -8,7 +8,7 @@ From iris.algebra Require Import excl.
 Definition spawn : val :=
   λ: "f",
     let: "c" := ref NONE in
-    Fork ("c" <- SOME ("f" #())) ;; "c".
+    Fork ("c" <- SOME ("f" ())) ;; "c".
 Definition join : val :=
   rec: "join" "c" :=
     match: !"c" with
@@ -49,7 +49,7 @@ Proof. solve_proper. Qed.
 Lemma spawn_spec (Ψ : val → iProp Σ) e (f : val) :
   to_val e = Some f →
   heapN ⊥ N →
-  {{{ heap_ctx ∗ WP f #() {{ Ψ }} }}} spawn e {{{ l, RET #l; join_handle l Ψ }}}.
+  {{{ heap_ctx ∗ WP f () {{ Ψ }} }}} spawn e {{{ l, RET LocV l; join_handle l Ψ }}}.
 Proof.
   iIntros (<-%of_to_val ? Φ) "(#Hh & Hf) HΦ". rewrite /spawn /=.
   wp_let. wp_alloc l as "Hl". wp_let.
@@ -64,7 +64,7 @@ Proof.
 Qed.
 
 Lemma join_spec (Ψ : val → iProp Σ) l :
-  {{{ join_handle l Ψ }}} join #l {{{ v, RET v; Ψ v }}}.
+  {{{ join_handle l Ψ }}} join l {{{ v, RET v; Ψ v }}}.
 Proof.
   rewrite /join_handle; iIntros (Φ) "[% H] HΦ". iDestruct "H" as (γ) "(#?&Hγ&#?)".
   iLöb as "IH". wp_rec. wp_bind (! _)%E. iInv N as (v) "[Hl Hinv]" "Hclose".
