theories/tests/tree_sum.v
@@ -12,7 +12,7 @@ Fixpoint is_tree `{!heapG Σ} (v : val) (t : tree) : iProp Σ :=
   | leaf n => ⌜v = InjLV #n⌝
   | node tl tr =>
      ∃ (ll lr : loc) (vl vr : val),
-       ⌜v = InjRV (#ll,#lr)⌝ ∗ ll ↦ vl ∗ is_tree vl tl ∗ lr ↦ vr ∗ is_tree vr tr
+       ⌜v = InjRV (ll,lr)⌝ ∗ ll ↦ vl ∗ is_tree vl tl ∗ lr ↦ vr ∗ is_tree vr tr
   end%I.
 
 Fixpoint sum (t : tree) : Z :=
@@ -34,8 +34,8 @@ Definition sum' : val := λ: "t",
   !"l".
 
 Lemma sum_loop_wp `{!heapG Σ} v t l (n : Z) (Φ : val → iProp Σ) :
-  heap_ctx -∗ l ↦ #n -∗ is_tree v t -∗ (l ↦ #(sum t + n) -∗ is_tree v t -∗ Φ #()) -∗
-  WP sum_loop v #l {{ Φ }}.
+  heap_ctx -∗ l ↦ #n -∗ is_tree v t -∗ (l ↦ #(sum t + n) -∗ is_tree v t -∗ Φ ()%V) -∗
+  WP sum_loop v l {{ Φ }}.
 Proof.
   iIntros "#Hh Hl Ht HΦ".
   iLöb as "IH" forall (v t l n Φ). wp_rec. wp_let.
