theories/heap_lang/lib/barrier/specification.v
@@ -10,10 +10,10 @@ Context `{!heapG Σ} `{!barrierG Σ}.
 Lemma barrier_spec (N : namespace) :
   heapN ⊥ N →
   ∃ recv send : loc → iProp Σ -n> iProp Σ,
-    (∀ P, heap_ctx ⊢ {{ True }} newbarrier #()
-                     {{ v, ∃ l : loc, ⌜v = #l⌝ ∗ recv l P ∗ send l P }}) ∧
-    (∀ l P, {{ send l P ∗ P }} signal #l {{ _, True }}) ∧
-    (∀ l P, {{ recv l P }} wait #l {{ _, P }}) ∧
+    (∀ P, heap_ctx ⊢ {{ True }} newbarrier ()
+                     {{ v, ∃ l : loc, ⌜v = l⌝ ∗ recv l P ∗ send l P }}) ∧
+    (∀ l P, {{ send l P ∗ P }} signal l {{ _, True }}) ∧
+    (∀ l P, {{ recv l P }} wait l {{ _, P }}) ∧
     (∀ l P Q, recv l (P ∗ Q) ={↑N}=> recv l P ∗ recv l Q) ∧
     (∀ l P Q, (P -∗ Q) -∗ recv l P -∗ recv l Q).
 Proof.
